theories/Metatheory.v
@@ -38,7 +38,8 @@ Qed.
 Lemma lift_distributes_over_bind:
   forall i k b ts c,
   lift i k (bind b ts c) =
-    bind (lift i (S k) b) (map (lift i k) ts) (lift i (k + length ts) c).
+    bind (lift i (S k) b) (traverse_list (lift i) k ts)
+      (lift i (k + length ts) c).
 Proof.
   auto.
 Qed.
@@ -125,10 +126,9 @@ Proof.
   - do 3 rewrite lift_distributes_over_negation; f_equal.
     induction H; simpl.
     + reflexivity.
-    + f_equal.
-      * do 3 rewrite traverse_list_length.
-        apply H; lia.
-      * assumption.
+    + f_equal; auto.
+      do 3 rewrite traverse_list_length.
+      apply H; lia.
   (* Case: jump. *)
   - do 3 rewrite lift_distributes_over_jump.
     f_equal; auto.
@@ -137,8 +137,12 @@ Proof.
   - do 3 rewrite lift_distributes_over_bind.
     f_equal; auto.
     + apply IHe1; lia.
-    + list induction over H.
-    + rewrite map_length.
+    + induction H; simpl.
+      * reflexivity.
+      * f_equal; auto.
+        do 3 rewrite traverse_list_length.
+        apply H; lia.
+    + rewrite traverse_list_length.
       apply IHe2; lia.
 Qed.
 
@@ -175,11 +179,10 @@ Proof.
   - do 4 rewrite lift_distributes_over_negation; f_equal.
     induction H; simpl.
     + reflexivity.
-    + f_equal.
-      * do 4 rewrite traverse_list_length.
-        replace (length l0 + (i + l)) with (i + (length l0 + l)); try lia.
-        apply H; lia.
-      * assumption.
+    + f_equal; auto.
+      do 4 rewrite traverse_list_length.
+      replace (length l0 + (i + l)) with (i + (length l0 + l)); try lia.
+      apply H; lia.
   (* Case: jump. *)
   - do 4 rewrite lift_distributes_over_jump.
     f_equal; auto.
@@ -189,8 +192,360 @@ Proof.
     f_equal; auto.
     + replace (S (i + l)) with (i + S l); auto.
       apply IHe1; lia.
-    + list induction over H.
-    + do 2 rewrite map_length.
+    + induction H; simpl.
+      * reflexivity.
+      * f_equal; auto.
+        do 4 rewrite traverse_list_length.
+        replace (length l0 + (i + l)) with (i + (length l0 + l)); try lia.
+        apply H; lia.
+    + do 2 rewrite traverse_list_length.
       rewrite plus_assoc_reverse.
       apply IHe2; lia.
+Qed.
+
+(** ** Substitution *)
+
+Lemma subst_distributes_over_negation:
+  forall y k ts,
+  subst y k (negation ts) =
+    negation (traverse_list (subst y) k ts).
+Proof.
+  auto.
+Qed.
+
+Lemma subst_distributes_over_jump:
+  forall y k x xs,
+  subst y k (jump x xs) =
+    jump (subst y k x) (map (subst y k) xs).
+Proof.
+  auto.
+Qed.
+
+Lemma subst_distributes_over_bind:
+  forall y k b ts c,
+  subst y k (bind b ts c) =
+    bind (subst y (S k) b) (traverse_list (subst y) k ts)
+      (subst y (k + length ts) c).
+Proof.
+  auto.
+Qed.
+
+Lemma subst_bound_gt:
+  forall e k n,
+  n > k -> subst e k n = pred n.
+Proof.
+  intros.
+  unfold subst; simpl.
+  destruct (lt_eq_lt_dec k n) as [ [ ? | ? ] | ? ].
+  (* Case: k < n. *)
+  - reflexivity.
+  (* Case: k = n. *)
+  - exfalso; lia.
+  (* Case: k > n. *)
+  - exfalso; lia.
+Qed.
+
+Lemma subst_bound_eq:
+  forall e k n,
+  n = k -> subst e k n = lift n 0 e.
+Proof.
+  intros.
+  unfold subst; simpl.
+  destruct (lt_eq_lt_dec k n) as [ [ ? | ? ] | ? ].
+  (* Case: k < n. *)
+  - exfalso; lia.
+  (* Case: k = n. *)
+  - congruence.
+  (* Case: k > n. *)
+  - exfalso; lia.
+Qed.
+
+Lemma subst_bound_lt:
+  forall e k n,
+  n < k -> subst e k n = n.
+Proof.
+  intros.
+  unfold subst; simpl.
+  destruct (lt_eq_lt_dec k n) as [ [ ? | ? ] | ? ].
+  (* Case: k < n. *)
+  - exfalso; lia.
+  (* Case: k = n. *)
+  - exfalso; lia.
+  (* Case: k > n. *)
+  - reflexivity.
+Qed.
+
+Lemma lift_addition_distributes_over_subst:
+  forall e y i p k,
+  lift i (p + k) (subst y p e) = subst (lift i k y) p (lift i (S (p + k)) e).
+Proof.
+  induction e using pseudoterm_deepind; intros.
+  (* Case: type. *)
+  - reflexivity.
+  (* Case: prop. *)
+  - reflexivity.
+  (* Case: base. *)
+  - reflexivity.
+  (* Case: void. *)
+  - reflexivity.
+  (* Case: bound. *)
+  - destruct (lt_eq_lt_dec p n) as [ [ ? | ? ] | ? ].
+    + destruct n; try lia.
+      destruct (le_gt_dec (p + k) n).
+      * rewrite lift_bound_ge; try lia.
+        rewrite subst_bound_gt; try lia.
+        rewrite lift_bound_ge; try lia.
+        rewrite subst_bound_gt; try lia.
+        f_equal; lia.
+      * rewrite lift_bound_lt; auto with arith.
+        rewrite subst_bound_gt; auto with arith.
+        rewrite lift_bound_lt; try lia.
+        rewrite subst_bound_gt; try lia.
+        reflexivity.
+    + destruct e.
+      rewrite lift_bound_lt; try lia.
+      rewrite subst_bound_eq; auto.
+      rewrite subst_bound_eq; auto.
+      symmetry; apply lift_lift_permutation; lia.
+    + rewrite lift_bound_lt; try lia.
+      rewrite subst_bound_lt; try lia.
+      rewrite subst_bound_lt; auto.
+      rewrite lift_bound_lt; try lia.
+      reflexivity.
+  (* Case: negation. *)
+  - rewrite lift_distributes_over_negation.
+    do 2 rewrite subst_distributes_over_negation.
+    rewrite lift_distributes_over_negation; f_equal.
+    induction H; simpl.
+    + reflexivity.
+    + f_equal; auto.
+      do 4 rewrite traverse_list_length.
+      replace (length l + (p + k)) with (length l + p + k); try lia.
+      replace (length l + S (p + k)) with (S (length l + p + k)); try lia.
+      apply H.
+  (* Case: jump. *)
+  - rewrite lift_distributes_over_jump.
+    do 2 rewrite subst_distributes_over_jump.
+    rewrite lift_distributes_over_jump.
+    f_equal; auto.
+    list induction over H.
+  (* Case: bind. *)
+  - rewrite lift_distributes_over_bind.
+    do 2 rewrite subst_distributes_over_bind.
+    rewrite lift_distributes_over_bind.
+    f_equal.
+    + replace (S (p + k)) with (S p + k); try lia.
+      apply IHe1.
+    + induction H; simpl.
+      * reflexivity.
+      * f_equal; auto.
+        do 4 rewrite traverse_list_length.
+        replace (length l + (p + k)) with (length l + p + k); try lia.
+        replace (length l + S (p + k)) with (S (length l + p + k)); try lia.
+        apply H.
+    + do 2 rewrite traverse_list_length.
+      replace (p + k + length ts) with (p + length ts + k); try lia.
+      replace (S (p + k) + length ts) with (S (p + length ts + k)); try lia.
+      apply IHe2.
+Qed.
+
+Lemma lift_distributes_over_subst:
+  forall a b i k,
+  lift i k (subst b 0 a) = subst (lift i k b) 0 (lift i (S k) a).
+Proof.
+  intros.
+  replace k with (0 + k); auto.
+  apply lift_addition_distributes_over_subst.
+Qed.
+
+Lemma subst_lift_simplification:
+  forall e y i p k,
+  p <= i + k ->
+  k <= p -> subst y p (lift (S i) k e) = lift i k e.
+Proof.
+  induction e using pseudoterm_deepind; intros.
+  (* Case: type. *)
+  - reflexivity.
+  (* Case: prop. *)
+  - reflexivity.
+  (* Case: base. *)
+  - reflexivity.
+  (* Case: void. *)
+  - reflexivity.
+  (* Case: bound. *)
+  - destruct (le_gt_dec k n).
+    + rewrite lift_bound_ge; auto.
+      rewrite lift_bound_ge; auto.
+      rewrite subst_bound_gt; try lia.
+      f_equal; lia.
+    + rewrite lift_bound_lt; auto.
+      rewrite lift_bound_lt; auto.
+      rewrite subst_bound_lt; auto.
+      lia.
+  (* Case: negation. *)
+  - do 2 rewrite lift_distributes_over_negation.
+    rewrite subst_distributes_over_negation.
+    f_equal; induction H; auto.
+    simpl; f_equal; auto.
+    do 3 rewrite traverse_list_length.
+    apply H; lia.
+  (* Case: jump. *)
+  - do 2 rewrite lift_distributes_over_jump.
+    rewrite subst_distributes_over_jump.
+    f_equal; auto.
+    list induction over H.
+  (* Case: bind. *)
+  - do 2 rewrite lift_distributes_over_bind.
+    rewrite subst_distributes_over_bind.
+    f_equal.
+    + apply IHe1; lia.
+    + induction H; auto.
+      simpl; f_equal; auto.
+      do 3 rewrite traverse_list_length.
+      apply H; lia.
+    + rewrite traverse_list_length.
+      apply IHe2; lia.
+Qed.
+
+Lemma lift_and_subst_commute:
+  forall e y i p k,
+  k <= p ->
+  lift i k (subst y p e) = subst y (i + p) (lift i k e).
+Proof.
+  induction e using pseudoterm_deepind; intros.
+  (* Case: type. *)
+  - reflexivity.
+  (* Case: prop. *)
+  - reflexivity.
+  (* Case: base. *)
+  - reflexivity.
+  (* Case: void. *)
+  - reflexivity.
+  (* Case: bound. *)
+  - destruct (lt_eq_lt_dec p n) as [ [ ? | ? ] | ? ]; simpl.
+    + rewrite lift_bound_ge; try lia.
+      rewrite subst_bound_gt; try lia.
+      rewrite lift_bound_ge; try lia.
+      rewrite subst_bound_gt; try lia.
+      f_equal; lia.
+    + rewrite lift_bound_ge; try lia.
+      rewrite subst_bound_eq; try lia.
+      rewrite subst_bound_eq; try lia.
+      apply lift_lift_simplification; lia.
+    + rewrite subst_bound_lt; auto.
+      destruct (le_gt_dec k n).
+      * rewrite lift_bound_ge; auto.
+        rewrite subst_bound_lt; try lia.
+        reflexivity.
+      * rewrite lift_bound_lt; auto.
+        rewrite subst_bound_lt; auto.
+        lia.
+  (* Case: negation. *)
+  - rewrite lift_distributes_over_negation.
+    do 2 rewrite subst_distributes_over_negation.
+    rewrite lift_distributes_over_negation.
+    f_equal; induction H; auto.
+    simpl; f_equal; auto.
+    do 4 rewrite traverse_list_length.
+    replace (length l + (i + p)) with (i + (length l + p)); try lia.
+    apply H; lia.
+  (* Case: jump. *)
+  - rewrite lift_distributes_over_jump.
+    do 2 rewrite subst_distributes_over_jump.
+    rewrite lift_distributes_over_jump.
+    f_equal; auto.
+    list induction over H.
+  (* Case: bind. *)
+  - rewrite lift_distributes_over_bind.
+    do 2 rewrite subst_distributes_over_bind.
+    rewrite lift_distributes_over_bind.
+    f_equal.
+    + replace (S (i + p)) with (i + S p); try lia.
+      apply IHe1; lia.
+    + induction H; auto.
+      simpl; f_equal; auto.
+      do 4 rewrite traverse_list_length.
+      replace (length l + (i + p)) with (i + (length l + p)); try lia.
+      apply H; lia.
+    + do 2 rewrite traverse_list_length.
+      replace (i + p + length ts) with (i + (p + length ts)); try lia.
+      apply IHe2; lia.
+Qed.
+
+Lemma subst_addition_distributes_over_itself:
+  forall e y z p k,
+  subst y (p + k) (subst z p e) = subst (subst y k z) p (subst y (S (p + k)) e).
+Proof.
+  induction e using pseudoterm_deepind; intros.
+  (* Case: type. *)
+  - reflexivity.
+  (* Case: prop. *)
+  - reflexivity.
+  (* Case: base. *)
+  - reflexivity.
+  (* Case: void. *)
+  - reflexivity.
+  (* Case: bound. *)
+  - destruct (lt_eq_lt_dec p n) as [ [ ? | ? ] | ? ].
+    + destruct n; try lia.
+      rewrite subst_bound_gt; try lia.
+      destruct (lt_eq_lt_dec (p + k) n) as [ [ ? | ? ] | ? ].
+      * rewrite subst_bound_gt; try lia.
+        rewrite subst_bound_gt; try lia.
+        rewrite subst_bound_gt; try lia.
+        reflexivity.
+      * rewrite subst_bound_eq; try lia.
+        rewrite subst_bound_eq; try lia.
+        rewrite subst_lift_simplification; try lia.
+        reflexivity.
+      * rewrite subst_bound_lt; try lia.
+        rewrite subst_bound_lt; try lia.
+        rewrite subst_bound_gt; try lia.
+        reflexivity.
+    + rewrite subst_bound_eq; try lia.
+      rewrite subst_bound_lt; try lia.
+      rewrite subst_bound_eq; try lia.
+      rewrite lift_and_subst_commute; try lia.
+      f_equal; lia.
+    + rewrite subst_bound_lt; try lia.
+      rewrite subst_bound_lt; try lia.
+      rewrite subst_bound_lt; try lia.
+      rewrite subst_bound_lt; try lia.
+      reflexivity.
+  (* Case: negation. *)
+  - do 4 rewrite subst_distributes_over_negation.
+    f_equal; induction H; auto.
+    simpl; f_equal; auto.
+    do 4 rewrite traverse_list_length.
+    replace (length l + (p + k)) with (length l + p + k); try lia.
+    replace (length l + S (p + k)) with (S (length l + p + k)); try lia.
+    apply H.
+  (* Case: jump. *)
+  - do 4 rewrite subst_distributes_over_jump.
+    f_equal; auto.
+    list induction over H.
+  (* Case: bind. *)
+  - do 4 rewrite subst_distributes_over_bind.
+    f_equal.
+    + replace (S (p + k)) with (S p + k); try lia.
+      apply IHe1; lia.
+    + induction H; auto.
+      simpl; f_equal; auto.
+      do 4 rewrite traverse_list_length.
+      replace (length l + (p + k)) with (length l + p + k); try lia.
+      replace (length l + S (p + k)) with (S (length l + p + k)); try lia.
+      apply H.
+    + do 2 rewrite traverse_list_length.
+      replace (p + k + length ts) with (p + length ts + k); try lia.
+      replace (S (p + k) + length ts) with (S (p + length ts + k)); try lia.
+      apply IHe2; lia.
+Qed.
+
+Lemma subst_distributes_over_itself:
+  forall a b c k,
+  subst c k (subst b 0 a) = subst (subst c k b) 0 (subst c (S k) a).
+Proof.
+  intros.
+  replace k with (0 + k); auto.
+  apply subst_addition_distributes_over_itself.
 Qed.
